Weidenbach_Book/IsaSAT.thy
@@ -923,12 +923,12 @@ lemma rewatch_st_correctness:
      correct_watching_init T)\<close>
   apply (rule SPEC_rule_conjI)
   subgoal
-    using rewatch_correctness[OF assms]
+    using Watched_Literals_Watch_List_Initialisation.rewatch_correctness[OF assms]
     unfolding rewatch_st_def
     apply (cases S, case_tac \<open>rewatch b g\<close>)
     by (auto simp: RES_RETURN_RES)
   subgoal
-    using rewatch_correctness[OF assms]
+    using Watched_Literals_Watch_List_Initialisation.rewatch_correctness[OF assms]
     unfolding rewatch_st_def
     apply (cases S, case_tac \<open>rewatch b g\<close>)
     by (force simp: RES_RETURN_RES)+
@@ -2765,10 +2765,10 @@ export_code IsaSAT_code
     Version.version
   in SML_imp module_name SAT_Solver file_prefix "IsaSAT_solver"
 
-external_file "code/Unsynchronized.sml"
-external_file "code/IsaSAT.mlb"
-external_file "code/IsaSAT.sml"
-external_file "code/dimacs_parser.sml"
+external_file \<open>code/Unsynchronized.sml\<close>
+external_file \<open>code/IsaSAT.mlb\<close>
+external_file \<open>code/IsaSAT.sml\<close>
+external_file \<open>code/dimacs_parser.sml\<close>
 
 export_generated_files _
 
@@ -2776,14 +2776,12 @@ compile_generated_files
    \<open>code/IsaSAT_solver.ML\<close>
   external_files
     \<open>code/IsaSAT.mlb\<close>
-    "code/Unsynchronized.sml"
-    "code/IsaSAT.mlb"
-    "code/IsaSAT.sml"
-    "code/dimacs_parser.sml"
+    \<open>code/Unsynchronized.sml\<close>
+    \<open>code/IsaSAT.sml\<close>
+    \<open>code/dimacs_parser.sml\<close>
   where \<open>fn dir =>
     let
       val exec = Generated_Files.execute (Path.append dir (Path.basic "code"));
-      val _ = exec \<open>ls\<close> "ls  >> /tmp/test"
       val _ = exec \<open>rename file\<close> "mv IsaSAT_solver.ML IsaSAT_solver.sml"
       val _ =
         exec \<open>Copy files\<close>
@@ -2792,7 +2790,8 @@ compile_generated_files
       val _ =
         exec \<open>Compilation\<close>
           (File.bash_path \<^path>\<open>$ISABELLE_MLTON\<close> ^
-            " -default-type int64 IsaSAT.mlb");
+            " -const 'MLton.safe false' -verbose 1 -default-type int64 -output IsaSAT " ^
+            " -codegen native -inline 700 -cc-opt -O3 IsaSAT.mlb");
       val _ =
         exec \<open>Copy binary files\<close>
           ("cp IsaSAT " ^
